WIP: draft of AIG -> CNF

LeanSAT/AIG/CNF.lean
@@ -1,26 +1,244 @@
 import LeanSAT.AIG.Basic
 import LeanSAT.Reflect.CNF.Basic
 import LeanSAT.Reflect.CNF.Relabel
+import LeanSAT.Reflect.CNF.Relabel
+import LeanSAT.Reflect.BoolExpr.Tseitin.Defs
+import LeanSAT.Reflect.BoolExpr.Tseitin.Lemmas
+
+abbrev CNFVar (env : Env) := Nat ⊕ (Fin env.decls.size)
+
+namespace Decl
+
+def constToCNF (output : α) (const : Bool) : CNF α :=
+  [[(output, const)]]
+
+def gateToCNF (output : α) (lhs rhs : α) (linv rinv : Bool) : CNF α :=
+    -- a ↔ (b and c) as CNF: (¬a ∨ b) ∧ (¬a ∨ c) ∧ (a ∨ ¬b ∨ ¬c)
+    -- a ↔ (b and ¬c) as CNF: (¬a ∨ b) ∧ (¬a ∨ ¬c) ∧ (a ∨ ¬b ∨ c)
+    -- a ↔ (¬b and c) as CNF: (¬a ∨ ¬b) ∧ (¬a ∨ c) ∧ (a ∨ b ∨ ¬c)
+    -- a ↔ (¬b and ¬c) as CNF: (¬a ∨ ¬b) ∧ (¬a ∨ ¬c) ∧ (a ∨ b ∨ c)
+   [
+     [(output, false), (lhs, !linv)],
+     [(output, false), (rhs, !rinv)],
+     [(output, true),  (lhs, linv), (rhs, rinv)]
+   ]
+
+@[simp]
+theorem constToCNF_eval :
+    (constToCNF output b).eval assign
+      =
+    (assign output == b) := by
+  simp [constToCNF, CNF.eval, CNF.Clause.eval]
+
+theorem constToCNF_sat :
+    (constToCNF output b).sat assign
+      ↔
+    (assign output = b) := by
+  simp [CNF.sat]
+
+@[simp]
+theorem gateToCNF_eval :
+    (gateToCNF output lhs rhs linv rinv).eval assign
+      =
+    (assign output == ((xor (assign lhs) linv) && (xor (assign rhs) rinv))) := by
+  simp [gateToCNF, CNF.eval, CNF.Clause.eval]
+  cases assign output
+    <;> cases assign lhs
+      <;> cases assign rhs
+        <;> cases linv
+          <;> cases rinv
+            <;> decide
+
+theorem gateToCNF_sat :
+    (gateToCNF output lhs rhs linv rinv).sat assign
+      ↔
+    (assign output = ((xor (assign lhs) linv) && (xor (assign rhs) rinv))) := by
+  simp [CNF.sat]
+
+end Decl
 
 namespace Env
 
+-- TODO: cache
 def toCNF (entry : Entrypoint) : CNF Nat :=
-  let cnf := go entry.env 0 ⟨entry.start, entry.inv⟩ (by omega) []
-  cnf.relabel fun | .inl var => var.val | .inr var => entry.env.decls.size + var
+  let baseCnf := go entry.env entry.start entry.inv []
+  let cnf : CNF (CNFVar entry.env) := [(.inr ⟨entry.start, entry.inv⟩, true)] :: baseCnf
+  cnf.relabel inj
 where
-  go (env : Env) (idx : Nat) (upper : Fin env.decls.size) (h : idx ≤ upper)
-      (curr : CNF ((Fin env.decls.size) ⊕ Nat)) : CNF ((Fin env.decls.size) ⊕ Nat) :=
-    let decl := env.decls[idx]'sorry
-    let declCnf : CNF ((Fin env.decls.size) ⊕ Nat) :=
-      match decl with
-      | .const b => sorry
-      | .atom a => sorry
-      | .gate lhs rhs linv rinv => sorry
-    let newCnf := curr ++ declCnf
-    if h2:idx = upper then
-       newCnf
-    else
-       go env (idx + 1) upper (by omega) newCnf
-  termination_by upper.val - idx
+  inj {env : Env} (var : CNFVar env) : Nat :=
+    match var with
+    | .inl var => env.decls.size + var
+    | .inr var => var.val
+  go (env : Env) (upper : Nat) (h : upper < env.decls.size) (cnf : CNF (CNFVar env)) : CNF (CNFVar env) :=
+    let decl := env.decls[upper]
+    let output := .inr ⟨upper, h⟩
+    match heq:decl with
+    | .const b => Decl.constToCNF output b ++ cnf
+    | .atom a => CNF.eq output (.inl a) ++ cnf
+    | .gate lhs rhs linv rinv =>
+      have := env.inv upper lhs rhs linv rinv h heq
+      let lCNF := go env lhs (by omega) cnf
+      let rCNF := go env rhs (by omega) lCNF
+      Decl.gateToCNF output (.inr ⟨lhs, (by omega)⟩) (.inr ⟨rhs, (by omega)⟩) linv rinv ++ rCNF
+
+theorem toCNF.inj_is_injection {env : Env} (a b : CNFVar env) :
+    toCNF.inj a = toCNF.inj b → a = b := by
+  intro h
+  cases a with
+  | inl =>
+    cases b with
+    | inl =>
+      dsimp [inj] at h
+      apply congrArg
+      apply Nat.add_left_cancel
+      exact h
+    | inr rhs =>
+      exfalso
+      dsimp [inj] at h
+      have := rhs.isLt
+      omega
+  | inr lhs =>
+    cases b with
+    | inl =>
+      exfalso
+      dsimp [inj] at h
+      have := lhs.isLt
+      omega
+    | inr =>
+      dsimp [inj] at h
+      apply congrArg
+      apply Fin.eq_of_val_eq
+      exact h
+
+-- TODO: simplify and move to basic theory
+theorem denote_idx_const (h : env.decls[start] = .const b) :
+    ⟦env, ⟨start, hstart⟩, assign⟧ = b := by
+  unfold denote denote.go
+  split <;> simp_all
+
+theorem denote_idx_atom (h : env.decls[start] = .atom a) :
+    ⟦env, ⟨start, hstart⟩, assign⟧ = assign a := by
+  unfold denote denote.go
+  split <;> simp_all
+
+theorem denote_idx_gate (h : env.decls[start] = .gate lhs rhs linv rinv) :
+    ⟦env, ⟨start, hstart⟩, assign⟧
+      =
+    (
+      (xor ⟦env, ⟨lhs, by have := env.inv start lhs rhs linv rinv hstart h; omega⟩, assign⟧ linv)
+        &&
+      (xor ⟦env, ⟨rhs, by have := env.inv start lhs rhs linv rinv hstart h; omega⟩, assign⟧ rinv)
+    ) := by
+  unfold denote
+  conv =>
+    lhs
+    unfold denote.go
+  split
+  . simp_all
+  . simp_all
+  . next heq =>
+    rw [h] at heq
+    simp_all
+
+theorem toCNF.go_commute (env : Env) (base) (rhs lhs) (hl) (hr) (assign) :
+    (go env rhs hr (go env lhs hl base)).eval assign
+      =
+    (go env lhs hl (go env rhs hr base)).eval assign := by
+  sorry
+
+theorem toCNF.denote_as_go (env : Env) (upper : Nat) (h1) (assign) (base) :
+    ((assign (.inr ⟨upper, h1⟩) == ⟦env, ⟨upper, h1⟩, (fun var => assign (.inl var))⟧) = false)
+      →
+    ((go env upper h1 base).eval assign = false) := by
+  intro h
+  unfold go
+  dsimp
+  split
+  . next b heq =>
+    rw [denote_idx_const heq] at h
+    simp [h]
+  . next a heq =>
+    rw [denote_idx_atom heq] at h
+    simp [h]
+  . next lhs rhs linv rinv heq =>
+    rw [denote_idx_gate heq] at h
+    simp
+    have := env.inv upper lhs rhs linv rinv h1 heq
+    match hl:(assign (.inr ⟨lhs, by omega⟩) == ⟦env, ⟨lhs, by omega⟩, fun var => assign (Sum.inl var)⟧) with
+    | true =>
+      match hr:(assign (.inr ⟨rhs, by omega⟩) == ⟦env, ⟨rhs, by omega⟩, fun var => assign (Sum.inl var)⟧) with
+      | true =>
+        simp at hl hr
+        rw [← hl, ← hr] at h
+        simp [h]
+      | false =>
+        have rih := toCNF.denote_as_go env rhs (by omega) assign (go env lhs (by omega) base) hr
+        simp [rih]
+    | false =>
+      have lih := toCNF.denote_as_go env lhs (by omega) assign (go env rhs (by omega) base) hl
+      rw [go_commute]
+      simp [lih]
+
+def mixAssigns {env : Env} (assign1 : Nat → Bool) (assign2 : Fin env.decls.size → Bool)
+    : CNFVar env → Bool
+  | .inl var => assign1 var
+  | .inr var => assign2 var
+
+-- TODO: simp theorems
+def toCNF.satAssignment (env : Env) (assign1 : Nat → Bool) : CNFVar env → Bool :=
+  mixAssigns assign1 (fun idx => ⟦env, ⟨idx.val, idx.isLt⟩, assign1⟧)
+
+theorem toCNF.go_sat (env : Env) (start : Nat) (h1 : start < env.decls.size) (assign1 : Nat → Bool)
+    (base : CNF (CNFVar env)) (hbase : base.sat (satAssignment env assign1)):
+    (go env start h1 base).sat (satAssignment env assign1) := by
+  unfold CNF.sat
+  unfold go
+  dsimp
+  split
+  . next b heq =>
+    simp [satAssignment, mixAssigns]
+    rw [denote_idx_const heq]
+    simpa using hbase
+  . next b heq =>
+    simp [satAssignment, mixAssigns]
+    rw [denote_idx_atom heq]
+    simpa using hbase
+  . next lhs rhs linv rinv heq =>
+    simp [satAssignment, mixAssigns]
+    rw [denote_idx_gate heq]
+    have := env.inv start lhs rhs linv rinv h1 heq
+    have lih := go_sat env lhs (by omega) assign1 base hbase
+    have rih := go_sat env rhs (by omega) assign1 (go env lhs (by omega) base) lih
+    simpa using rih
+
+theorem toCNF.go_as_denote (env : Env) (start) (h1) (assign1) :
+    ((⟦env, ⟨start, h1⟩, assign1⟧ && (go env start h1 []).eval (satAssignment env assign1)) = false)
+      →
+    (⟦env, ⟨start, h1⟩, assign1⟧ = false) := by
+  intro h
+  rw [go_sat env start h1 assign1 [] (by simp)] at h
+  simpa using h
+
+theorem toCNF_equisat (entry : Entrypoint) : entry.unsat ↔ (toCNF entry).unsat := by
+  dsimp [toCNF]
+  rw [CNF.unsat_relabel_iff]
+  . constructor
+    . simp [CNF.unsat, CNF.eval_succ, Entrypoint.unsat]
+      intro h assign
+      specialize h (fun var => assign (.inl var))
+      match h2:assign (.inr ⟨entry.start, entry.inv⟩) with
+      | true =>
+        simp
+        apply toCNF.denote_as_go
+        rw [h]
+        simp [h2]
+      | false => simp
+    . intro h assign1
+      specialize h (toCNF.satAssignment entry.env assign1)
+      apply toCNF.go_as_denote
+      simpa using h
+  . intro a b _ _ hinj
+    apply toCNF.inj_is_injection
+    assumption
 
 end Env
